\documentclass[a4paper, 12pt]{article}

\usepackage{cmap}
\usepackage[T2A]{fontenc}
\usepackage[english, russian]{babel}
\usepackage[utf8]{inputenc}
\usepackage[left=2cm,right=1.5cm,top=2cm,bottom=2cm]{geometry}
% \usepackage{mathtext}
\usepackage{amsmath}
\usepackage{amssymb}
\usepackage{etoolbox}
\usepackage{amsthm}
% \usepackage{nicematrix}
% \usepackage{graphicx}
% \usepackage{tikz}
% \usepackage{parskip}
% \graphicspath{/Images/}

%Реализация aug, overbrace и underbrace без nice matrix
\newcommand\aug{\fboxsep=-\fboxrule\!\!\!\fbox{\strut}\!\!\!}
\newcommand\undermat[2]{\makebox[0pt][l]{$\smash{\underbrace
{\phantom{\begin{matrix}#2\end{matrix}}}_{\text{$#1$}}}$}#2}
\newcommand\overmat[2]{\makebox[0pt][l]{$\smash{\overbrace
{\phantom{\begin{matrix}#2\end{matrix}}}^{\text{$#1$}}}$}#2}
\newcommand\tab[1][.5cm]{\hspace*{#1}}
\newcommand\Underset[2]{\underset{\textstyle #1}{#2}}
\newcommand\Overset[2]{\overset{\textstyle #1}{#2}}


\theoremstyle{definition}
\newtheorem*{definition}{Определение}
\newtheorem*{theorem}{Теорема}
\newtheorem*{consequense}{Следствие}
\newtheorem*{lemma}{Лемма}
\newtheorem*{subtheorem}{Утверждение}
\newtheorem*{remark}{Замечание}


\begin{document}
    \fontsize{5pt}{5pt}\selectfont
    \begin{tabular}{l l l}
        $\tab[-0.2cm]\int \frac{dx}{a^2 + x^2} = \frac{1}{a}arctg \frac{x}{a}\ (a>0)$ & 
        $\int \frac{dx}{a^2 - x^2} = \frac{1}{2a}\ln \frac{|a + 1|}{|a - x|}$ & 
        $\int \frac{dx}{\sqrt{a^2 - x^2}} = \arcsin \frac{x}{a}$\\
        $\tab[-0.2cm]\int \frac{dx}{\sqrt{x^2 \pm a^2}} = \ln|x + \sqrt{x^2 \pm a^2}|$ & 
        $\int \frac{dx}{sh^2 x} = -\cth x$  &
        $\int \frac{dx}{ch^2 x} = \th x$
    \end{tabular}

    $\int \frac{P_n(x)}{Q_m(x)}dx = \frac{P_{m-k-1}}{Q_{m-k}} + \int \frac{R_{k-1}(x)}{Q_k(x)}dx$

    $\int \frac{P_n(x)}{y}dx = Q_{n-1}(x)y + \lambda\int \frac{dx}{y},\ y = \sqrt{ax^2 + by + c}$

    $t = \frac{x + a}{x + b} \Longrightarrow dt = \frac{(b-a)dx}{(x + b)^2}$ ИЛИ $x = \frac{bt - a}{t - 1} \Longrightarrow x + a = \frac{(a - b)t}{t - 1}$ и $x + b = \frac{a - b}{t - 1} $   
    
    $t = \tg \frac{x}{2},\ \sin x = \frac{2t}{1 + t^2},\ \cos x = \frac{1 - t^2}{1 + t^2}$

    $\int \frac{a_1\sin x + b_1\cos x + c_1}{a\sin x + b\cos y + c}dx = Ax + B\ln|a\sin x + b\cos y + c| + C\int \frac{dx}{a\sin x + b\cos y + c} $

    $\int\sin^nxdx = -\frac{1}{n}\cos x\sin^{n-1} x + 
    \frac{n-1}{n}\int\sin^{n-2}xdx$

    $\int\cos^nxdx = \frac{1}{n}\sin x\cos^{n-1} x + 
    \frac{n-1}{n}\int\cos^{n-2}xdx$ 

    \tab[1cm]\\
    \tab[1cm]\\
    \tab[1cm]\\
    \tab[1cm]\\
    \tab[1cm]\\
    \tab[1cm]

    $\int_{0}^{\frac{\pi}{2}} f(\sin x)dx = \int_{0}^{\frac{\pi}{2}} f(\cos x)dx$\tab[1cm]
    $\int_{0}^{\pi} xf(\sin x)dx = \frac{\pi}{ 2} \int_{0}^{\pi} f(\sin x)dx$

    $F(x) = \int_{\varphi_1(x)}^{\varphi_2(x)} f(t)dt \Longrightarrow F'(x) = f(\varphi_2(x))\varphi'_2(x) - f(\varphi_1(x))\varphi'_1(x)$
    
    $S = \int_{T_0}^{T_1} x(t)y'(t)dt = -\int_{T_0}^{T_1} x'(t)y(t)dt = \frac{1}{2}\int_{\alpha}^{\beta} r^2(\varphi)d \varphi$
    
    $V_{ox} = \pi \int_{a}^{b}f^2(x)dx = \pi \int_{a}^{b} y^2(x)x'dt$ 

    $V_{oy} = \pi \int_{a}^{b} f(x)dx^2 = 2\pi \int_{t_1}^{t_2} x(t)y(t)dx(t)$ 

    $|\Gamma| = \int_{T_0}^{T_1} \sqrt{(x'(t))^2 + (y'(t))^2 + (z'(t))^2}dt$
    
    $|\Gamma| = \int_{a}^{b} \sqrt{1 + (y')^2}dx$
    
    $|\Gamma| = \int_{\alpha}^{\beta} \sqrt{(r(\varphi))^2 + (r'(\varphi))^2}d \varphi =$
    $ \int_{\alpha}^{\beta} \sqrt{r^2\cdot (\varphi')^2 + (r')^2}\cdot sgn(\varphi')d \varphi$ 
    
\end{document}